$ H eq.triple p^2 + V $

$ angle.l x^n (d V)/(d x) angle.r = 2 n E angle.l x^(n - 1) angle.r - 2 n angle.l V x^(n - 1) angle.r $

$ angle.l (d V)/(d x) e^(n x) angle.r = 2 n E angle.l e^(n x) angle.r - 2 n angle.l V e^(n x) angle.r $

$ angle.l (d V)/(d x) e^(m x) x^n angle.r = 2 E angle.l m e^(m x) x^n + n e^(m x) x^(n - 1) angle.r - 2 angle.l V(m e^(m x) x^n + n e^(m x) x^(n - 1)) angle.r $
 
$ n angle.l (d V)/(d x) x^m p^(n - 1) angle.r = 2 E m angle.l x^(m - 1) p^(n - 1) angle.r - 2 m angle.l V x^(m - 1) p^(n - 1) angle.r $

$ E angle.l x^m p^n angle.r = angle.l x^m p^(n + 2) angle.r + angle.l V x^m p^n angle.r $

$ n angle.l (d V)/(d x) e^(i m theta) p^(n - 1) angle.r = 2 i m E angle.l e^(i m theta) p^(n - 1) angle.r - 2 i m angle.l V e^(i m theta) p^(n - 1) angle.r $

$ E angle.l e^(i m theta) p^n angle.r = angle.l e^(i m theta) p^(n + 2) angle.r + angle.l V e^(i m theta) p^n angle.r $

= Trigonometric potential
$ V = e^(i theta) + e^(-i theta) $
$ (n + 2m - 1) angle.l e^(i m theta) p^n angle.r = 2(m - 1)E angle.l e^(i(m - 1) theta) p^n angle.r + (n - 2m + 3) angle.l e^(i(m - 2)theta) p^n angle.r $
$ (2m - 1) angle.l e^(i m theta) angle.r = 2(m - 1)E angle.l e^(i(m - 1)theta) angle.r + (3 - 2m) angle.l e^(i(m - 2)theta) angle.r $
$ E angle.l e^(i m theta) p^n angle.r = angle.l e^(i m theta) p^(n + 2) angle.r + angle.l e^(i(m + 1)theta) p^n angle.r + angle.l e^(i(m - 1)theta) p^n angle.r $

= Coulomb potentia
$ V = -1/r + 1/r^2 $
$ 2(m + 1)E f(m, n) = 2(m - n)f(m - 2, n) + (n - 2m - 1)f(m - 1, n) $
$ E f(m, n - 2) = f(m, n) - f(m - 1, n - 2) + f(m - 2, n - 2) $

= Toda
$ V = e^x + e^(-x) $
